ground_zero/algebra/core.lean
@@ -1,0 +1,71 @@
+import ground_zero.structures ground_zero.types.integer
+open ground_zero.types.eq (pointed)
+open ground_zero.structures (hset)
+open ground_zero.types
+
+hott theory
+
+namespace ground_zero.algebra
+
+universes u v
+class magma (α : Type u) :=
+(mul : α → α → α)
+
+infixr ` · `:70 := magma.mul
+
+class pointed_magma (α : Type u) extends magma α :=
+(e {} : α)
+open pointed_magma
+
+class monoid (α : Type u) extends pointed_magma α :=
+(right_unit : Π (x : α), x · e = x)
+(left_unit : Π (x : α), e · x = x)
+(assoc : Π (x y z : α), x · (y · z) = (x · y) · z)
+
+class group (α : Type u) extends monoid α :=
+(inv : α → α)
+(right_inv : Π (x : α), x · inv x = e)
+(left_inv : Π (x : α), inv x · x = e)
+
+instance {α : Type u} [pointed_magma α] : has_one α := ⟨e⟩
+instance {α : Type u} [group α] : has_inv α := ⟨group.inv⟩
+
+def group.natural_pow {α : Type u} [group α] (x : α) : ℕ → α
+| 0 := 1
+| (n + 1) := x · group.natural_pow n
+
+def group.pow {α : Type u} [group α] (x : α) : integer → α
+| (integer.pos n) := group.natural_pow x n
+| (integer.neg n) := group.natural_pow x⁻¹ (n + 1)
+
+section
+  variables {α : Type u} [group α]
+  instance nat_pow : has_pow α ℕ := ⟨group.natural_pow⟩
+  instance int_pow : has_pow α integer := ⟨group.pow⟩
+end
+
+instance : magma bool := ⟨bxor⟩
+instance : pointed_magma bool := ⟨ff⟩
+
+instance : monoid bool :=
+{ right_unit := begin intro x, cases x; reflexivity end,
+  left_unit := begin intro x, cases x; reflexivity end,
+  assoc := begin intros x y z, cases x; cases y; cases z; reflexivity end }
+
+instance : group bool :=
+{ inv := id,
+  left_inv := begin intro x, cases x; reflexivity end,
+  right_inv := begin intro x, cases x; reflexivity end }
+
+def coeffspace (α : Type u) (β : Type v) :=
+β → α → α
+
+def is_eigenvalue {α : Type u} {β : Type v}
+  (mul : coeffspace α β) (A : α → α) (x : α) :=
+Σ y, A x = mul y x
+
+def spectrum {α : Type u} {β : Type v}
+  (mul : coeffspace α β) (A : α → α) :=
+Σ x, is_eigenvalue mul A x
+
+end ground_zero.algebra
